$\mathbf{3.23}$
	$a.$ $\mathrm{-8+18i}$
	$b.$ $\mathrm{\frac{2}{17}-\frac{3i}{17}}$
	$\textit{c.}$ $\mathrm{\frac{6}{25}-\frac{8i}{25}}$
	$\textit{d.}$  $\frac{34}{41}+\frac{22i}{41}$
	$\textit{e.}$ $\mathrm{i}$
	$\textit{f.}$ $\mathrm{1+i}$
$\mathbf{3.24}$ $\mathrm{6i}$
$\mathbf{3.25}$ $\mathrm{\frac{2}{5}}+\frac{i}{5}$
$\mathbf{3.26}$ $\mathrm{-\frac{3}{5}+\frac{i}{5}}$
$\mathbf{3.27}$ $\mathrm{-z:3rd,\overline{z}: 4th,-\overline{z}:2nd}$ 
$\mathbf{3.28}$ $
	$a.$ $\mathrm{w \overline{z}+\overline{w}z=wz+\overline{wz} \implies w\overline{z}+\overline{z}w \in \mathbb{R} }$
	$b.$ $\mathrm{w \overline{z}-\overline{w}z=2*\mathrm{Im} \implies w\overline{z}-\overline{z}w \in \mathbb{R} }$
$\mathbf{3.29}$ $\mathrm{3 \pm 2i}$
$\mathbf{3.30}$ $5, -4$ 
$\mathbf{3.31}$ $12\pi$
$\mathbf{3.32}$ $\mathrm{C}$
$\mathbf{3.33}$ $\mathrm{y=3x-1 \text{ wherein } z=x+iy}$
$\mathbf{3.34}$ 

**Hypothesis:** $(a+bi)(c+di)∈ \mathbb{R}$ 
**Conclusion:** $(b+ai)(d+ci)∈\mathbb{R}$
1. $(a+bi)(c+di)=(ac−bd)+(ad+bc)i$ 
2. $\text{Let } z \in \mathbb{C} \implies z \in \mathbb{R} \iff \mathrm{Im}(z)=0$
3. $\therefore \mathrm{Im}((a+bi)(c+di))=0 \implies ad+bc=0$
4. $\text{From the conclusion's expression:}$ $(b+ai)(d+ci)=(bd−ac)+(bc+ad)i$ 
5. $\mathrm{Im}((b+ai)(d+ci))=bc+ad$ 
6. $\text{From (3)} \because \text{Addition is communative}:bc+ad=ad+bc=0$ 
7. $\implies \mathrm{Im}((b+ai)(d+ci))=0$
8. $\therefore \text{ by (2):}$ $(b+ai)(d+ci)∈ \mathbb{R}$ 
9. QED

$\mathbf{3.35}$
	$a.$ $z=(x,-4)$
	$b.$ $y=\frac{1}{4}x+2$
	$c.$ $(x-3.5)^2+(y-0.5)^2=4$
$\mathbf{3.36}$ check paper
$\mathbf{3.37}$ $0$
$\mathbf{3.38}$ $(1-1)^2+(1+1)^2=4$
