$\mathbf{3.3.1}$ $\mathrm{260}$
$\mathbf{3.3.3}$ $\mathrm{|a+bi|=\sqrt{a^2 +b^2  }, |\overline{a-bi }|=\sqrt{ a^2+(-b^2) }=\sqrt{ a^2+b^2}}|$
$\mathbf{3.3.4}$ $4
	$a.$ $\mathrm{1+i}$
	$b.$ $\mathrm{3-2i}$
	$c.$ $\mathrm{-5+i}$
$\mathbf{3.3.5}$ 
	$a.$ $\frac{1}{5}$
	$b.$ $\frac{1}{5}$
	$c.$ $\mathrm{\frac{2 \sqrt{ 6 }}{13}}$
	$d.$ $\frac{13}{5}$ 
$\mathbf{3.3.6}$ $\mathrm{\left\{  z / \overline{z} \in \mathbb{I} | a=0 \text{ and } b \neq {0} \right\}},$  $\mathrm{\left\{  z / \overline{z} \in \mathbb{I} | b=0 \text{ and } a \neq {0} \right\}}$
